Matroid/Parallel.lean
@@ -1,0 +1,421 @@
+import Matroid.ForMathlib.SetPartition
+import Matroid.ForMathlib.Logic.Equiv.Set
+import Matroid.Flat
+
+open Set Set.Notation
+
+namespace Matroid
+
+variable {α : Type*} {M N : Matroid α} {e f g : α} {I X P D : Set α}
+
+section Parallel
+
+/-- The partition of the nonloops of `M` into parallel classes. -/
+def parallelClasses (M : Matroid α) : Partition {e | M.Nonloop e} :=
+  (M.cl_flat ∅).covbyPartition.congr M.setOf_nonloop_eq.symm
+
+def Parallel (M : Matroid α) : α → α → Prop := M.parallelClasses.Rel
+
+theorem parallel_iff : M.Parallel e f ↔ M.Nonloop e ∧ M.Nonloop f ∧ M.cl {e} = M.cl {f} := by
+  simp [Parallel, parallelClasses, and_comm (a := _ ∈ M.E), nonloop_iff_mem_compl_loops]
+
+instance {M : Matroid α} : IsSymm α M.Parallel :=
+  inferInstanceAs <| IsSymm α M.parallelClasses.Rel
+
+instance {M : Matroid α} : IsTrans α M.Parallel :=
+  inferInstanceAs <| IsTrans α M.parallelClasses.Rel
+
+theorem Parallel.symm (h : M.Parallel e f) : M.Parallel f e :=
+  Partition.Rel.symm h
+
+theorem parallel_comm : M.Parallel e f ↔ M.Parallel f e :=
+  Partition.rel_comm
+
+theorem Parallel.trans (h : M.Parallel e f) (h' : M.Parallel f g) : M.Parallel e g :=
+  Partition.Rel.trans h h'
+
+theorem Parallel.cl_eq_cl (h : M.Parallel e f) : M.cl {e} = M.cl {f} :=
+  (parallel_iff.1 h).2.2
+
+theorem Parallel.nonloop_left (h : M.Parallel e f) : M.Nonloop e :=
+  (parallel_iff.1 h).1
+
+theorem Parallel.nonloop_right (h : M.Parallel e f) : M.Nonloop f :=
+  h.symm.nonloop_left
+
+@[aesop unsafe 20% (rule_sets := [Matroid])]
+theorem Parallel.mem_ground_left (h : M.Parallel e f) : e ∈ M.E :=
+  h.nonloop_left.mem_ground
+
+@[aesop unsafe 20% (rule_sets := [Matroid])]
+theorem Parallel.mem_ground_right (h : M.Parallel e f) : f ∈ M.E :=
+  h.nonloop_right.mem_ground
+
+theorem Nonloop.parallel_iff_cl_eq_cl (he : M.Nonloop e) :
+    M.Parallel e f ↔ M.cl {e} = M.cl {f} := by
+  rw [Parallel, parallelClasses, Partition.rel_congr,
+    (M.cl_flat ∅).rel_covbyPartition_iff' ⟨he.mem_ground, he.not_loop⟩]; simp
+
+theorem Parallel.mem_cl (h : M.Parallel e f) : e ∈ M.cl {f} := by
+  rw [← h.cl_eq_cl]; exact mem_cl_of_mem' _ rfl
+
+theorem Parallel.parallel_iff_left (h : M.Parallel e f) {x : α} :
+    M.Parallel x e ↔ M.Parallel x f :=
+  ⟨fun h' ↦ h'.trans h , fun h' ↦ h'.trans h.symm⟩
+
+theorem Parallel.parallel_iff_right (h : M.Parallel e f) {x : α} :
+    M.Parallel e x ↔ M.Parallel f x :=
+  ⟨h.symm.trans, h.trans⟩
+
+theorem setOf_parallel_eq_cl_diff_loops (M : Matroid α) (e : α) :
+    {f | M.Parallel e f} = M.cl {e} \ M.cl ∅ := by
+  by_cases he : M.Nonloop e
+  · rw [Parallel, parallelClasses, Partition.rel_congr,
+      Partition.setOf_rel_eq_partOf, (M.cl_flat ∅).partOf_covbyPartition_eq,
+      cl_insert_cl_eq_cl_insert, insert_emptyc_eq]
+  rw [not_nonloop_iff_cl.1 he, diff_self, eq_empty_iff_forall_not_mem]
+  exact fun f hf ↦ he (Parallel.nonloop_left hf)
+
+theorem cl_eq_parallel_class_union_loops (M : Matroid α) (e : α) :
+    M.cl {e} = {f | M.Parallel e f} ∪ M.cl ∅ := by
+  rw [setOf_parallel_eq_cl_diff_loops, diff_union_self,
+    union_eq_self_of_subset_right (M.cl_mono (empty_subset _))]
+
+theorem Nonloop.parallel_self (h : M.Nonloop e) : M.Parallel e e :=
+  (h.parallel_iff_cl_eq_cl).2 rfl
+
+@[simp] theorem parallel_self_iff : M.Parallel e e ↔ M.Nonloop e :=
+  ⟨Parallel.nonloop_left, Nonloop.parallel_self⟩
+
+theorem Loop.not_parallel (h : M.Loop e) (f : α) : ¬ M.Parallel e f :=
+  fun h' ↦ h'.nonloop_left.not_loop h
+
+theorem Nonloop.parallel_iff_mem_cl (he : M.Nonloop e) : M.Parallel e f ↔ e ∈ M.cl {f} := by
+  refine ⟨Parallel.mem_cl, fun h ↦ ?_⟩
+  rw [cl_eq_parallel_class_union_loops, mem_union,  mem_setOf_eq, parallel_comm] at h
+  exact h.elim id (fun h' ↦ (he.not_loop h').elim)
+
+theorem Loopless.parallel_class_eq_cl (h : M.Loopless) (e : α) :
+    {f | M.Parallel e f} = M.cl {e} := by
+  rw [setOf_parallel_eq_cl_diff_loops, h.cl_empty, diff_empty]
+
+theorem Parallel.dep_of_ne (h : M.Parallel e f) (hne : e ≠ f) : M.Dep {e,f} := by
+  rw [pair_comm, ← h.nonloop_left.indep.mem_cl_iff_of_not_mem hne.symm]; exact h.symm.mem_cl
+
+theorem parallel_iff_circuit (hef : e ≠ f) : M.Parallel e f ↔ M.Circuit {e,f} := by
+  refine' ⟨fun h ↦ circuit_iff_dep_forall_diff_singleton_indep.2 ⟨h.dep_of_ne hef,_⟩, fun h ↦ _⟩
+  · rintro x (rfl | rfl)
+    · rw [pair_diff_left hef]; exact h.nonloop_right.indep
+    · rw [pair_diff_right hef]; exact h.nonloop_left.indep
+  rw [Nonloop.parallel_iff_mem_cl]
+  · convert h.mem_cl_diff_singleton_of_mem (mem_insert _ _); rw [pair_diff_left hef]
+  apply h.nonloop_of_mem_of_one_lt_card _ (mem_insert _ _)
+  rw [encard_pair hef]
+  norm_num
+
+theorem Parallel.circuit_of_ne (hef : M.Parallel e f) (hne : e ≠ f) : M.Circuit {e,f} := by
+  rwa [parallel_iff_circuit hne] at hef
+
+theorem Nonloop.parallel_iff_dep (he : M.Nonloop e) (hf : M.Nonloop f) (hef : e ≠ f) :
+    M.Parallel e f ↔ M.Dep {e,f} := by
+  rw [← hf.indep.mem_cl_iff_of_not_mem hef, he.parallel_iff_mem_cl]
+
+theorem Parallel.eq_of_indep (h : M.Parallel e f) (hi : M.Indep {e,f}) : e = f := by
+  by_contra hef
+  exact ((h.nonloop_left.parallel_iff_dep h.nonloop_right hef).1 h).not_indep hi
+
+theorem parallel_iff_nonloop_nonloop_indep_imp_eq :
+    M.Parallel e f ↔ M.Nonloop e ∧ M.Nonloop f ∧ (M.Indep {e,f} → e = f) := by
+  refine ⟨fun h ↦ ⟨h.nonloop_left, h.nonloop_right, fun hi ↦ h.eq_of_indep hi⟩, fun h ↦ ?_⟩
+  obtain (rfl | hne) := eq_or_ne e f
+  · exact h.1.parallel_self
+  rw [h.1.parallel_iff_dep h.2.1 hne, Dep, pair_subset_iff, and_iff_left h.2.1.mem_ground,
+    and_iff_left h.1.mem_ground]
+  exact fun hi ↦ hne (h.2.2 hi)
+
+theorem Parallel.loop_of_contract (hef : M.Parallel e f) (hne : e ≠ f) : (M ／ e).Loop f := by
+  rw [loop_iff_mem_cl_empty, contract_elem, contract_loops_eq, mem_diff]
+  exact ⟨hef.symm.mem_cl, hne.symm⟩
+
+end Parallel
+
+section Parallel'
+
+/-- Two elements are `Parallel'` if they are either both loops or are `Parallel` nonloops.
+(Sometimes allowing loops is more convenient.) -/
+def Parallel' (M : Matroid α) (e f : α) : Prop := e ∈ M.E ∧ f ∈ M.E ∧ M.cl {e} = M.cl {f}
+
+@[aesop unsafe 20% (rule_sets := [Matroid])]
+theorem Parallel'.mem_ground_left (h : M.Parallel' e f) : e ∈ M.E := h.1
+
+@[aesop unsafe 20% (rule_sets := [Matroid])]
+theorem Parallel'.mem_ground_right (h : M.Parallel' e f) : f ∈ M.E := h.2.1
+
+theorem Parallel'.cl_eq_cl (h : M.Parallel' e f) : M.cl {e} = M.cl {f} := h.2.2
+
+theorem Parallel'.symm (h : M.Parallel' e f) : M.Parallel' f e :=
+  ⟨h.mem_ground_right, h.mem_ground_left, h.cl_eq_cl.symm⟩
+
+theorem parallel'_self (h : e ∈ M.E) : M.Parallel' e e :=
+    ⟨h,h,rfl⟩
+
+theorem Parallel'.trans (h : M.Parallel' e f) (h' : M.Parallel' f g) : M.Parallel' e g :=
+  ⟨h.mem_ground_left, h'.mem_ground_right, h.cl_eq_cl.trans h'.cl_eq_cl⟩
+
+theorem Parallel'.parallel_of_nonloop (h : M.Parallel' e f) (he : M.Nonloop e) :
+    M.Parallel e f := by
+  rwa [Nonloop.parallel_iff_cl_eq_cl, h.cl_eq_cl]
+
+theorem Parallel.parallel' (h : M.Parallel e f) : M.Parallel' e f :=
+  ⟨h.mem_ground_left, h.mem_ground_right, h.cl_eq_cl⟩
+
+theorem Parallel'.parallel_iff (h : M.Parallel' e f) : M.Parallel e f ↔ M.Nonloop e :=
+  ⟨fun h' ↦ h'.nonloop_left, h.parallel_of_nonloop⟩
+
+theorem Parallel'.loop_of_loop (h : M.Parallel' e f) (he : M.Loop e) : M.Loop f := by
+  have h' := h.cl_eq_cl
+  rw [he.cl, eq_comm] at h'
+  rwa [loop_iff_cl_eq_cl_empty h.mem_ground_right]
+
+theorem Parallel'.loop_or_parallel (h : M.Parallel' e f) :
+    (M.Loop e ∧ M.Loop f) ∨ M.Parallel e f := by
+  obtain (he | he) := M.loop_or_nonloop e
+  · exact .inl ⟨he, h.loop_of_loop he⟩
+  exact .inr <| h.parallel_of_nonloop he
+
+theorem parallel'_iff_loops_or_parallel :
+    M.Parallel' e f ↔ (M.Loop e ∧ M.Loop f) ∨ M.Parallel e f := by
+  refine ⟨Parallel'.loop_or_parallel, ?_⟩
+  rintro (⟨he, hf⟩ | hef)
+  · rw [Matroid.Parallel', he.cl, hf.cl]
+    simp [he.mem_ground, hf.mem_ground]
+  exact hef.parallel'
+
+theorem parallel'_iff_cl_eq_cl (e f : α) (he : e ∈ M.E := by aesop_mat)
+    (hf : f ∈ M.E := by aesop_mat) : M.Parallel' e f ↔ M.cl {e} = M.cl {f} := by
+  rw [Matroid.Parallel', and_iff_right he, and_iff_right hf]
+
+theorem Parallel'.mem_cl (h : M.Parallel' e f) : e ∈ M.cl {f} := by
+  rw [← h.cl_eq_cl]
+  apply mem_cl_self _ _ h.mem_ground_left
+
+theorem Parallel'.eq_of_indep (h : M.Parallel' e f) (hef : M.Indep {e,f}) : e = f :=
+  (h.parallel_of_nonloop <| hef.nonloop_of_mem (.inl rfl)).eq_of_indep hef
+
+@[simp] theorem parallel'_iff_parallel [Loopless M] : M.Parallel' e f ↔ M.Parallel e f := by
+  rw [parallel'_iff_loops_or_parallel, or_iff_right (fun h ↦ M.not_loop e h.1)]
+
+end Parallel'
+
+section Iso
+
+/-
+We show if `φ` is a function with `Parallel' e (φ e)` for all `e`,
+then `φ` determines various matroid isomorphisms.
+There are a few different contexts, depending on whether `φ` is defined on all of `α` or
+only on a subtype, and whether or not `φ` is an equivalence.
+-/
+
+theorem cl_range_of_forall_parallel'_subtype {X : Set α} (φ : X → α)
+    (h_para : ∀ e : X, M.Parallel' e (φ e)) : M.cl (range φ) = M.cl X := by
+  simpa using M.cl_iUnion_congr (fun e ↦ {φ e}) (fun e ↦ {e.1}) (fun e ↦ (h_para e).cl_eq_cl.symm)
+
+theorem cl_image_of_forall_parallel'_subtype {X : Set α} (φ : X → α)
+    (h_para : ∀ e : X, M.Parallel' e (φ e)) (Y : Set X) : M.cl (φ '' Y) = M.cl Y := by
+  convert M.cl_biUnion_congr (fun e : X ↦ {φ e}) (fun e ↦ {e.1}) Y
+    (fun e _ ↦ (h_para e).cl_eq_cl.symm) <;> aesop
+
+theorem cl_image_of_forall_parallel' (φ : α → α) (h_para : ∀ e, M.Parallel' e (φ e))
+    (X : Set α) : M.cl (φ '' X) = M.cl X := by
+  rw [← cl_range_of_forall_parallel'_subtype (fun x : X ↦ φ x) (fun x ↦ h_para x), image_eq_range]
+
+/-- If `φ : X ≃ Y` is such that `e` and `φ e` are always `Parallel'`, then `φ` determines a
+matroid isomorphism between `M ↾ X` and `M ↾ Y`. -/
+def isoOfMapParallelRestr {X Y : Set α} (φ : X ≃ Y) (h_para : ∀ e : X,  M.Parallel' e (φ e)) :
+    (M ↾ X) ≂ (M ↾ Y) :=
+  isoOfForallImageCl φ
+  ( by
+      have hXE : X ⊆ M.E := fun x hx ↦ (h_para ⟨x,hx⟩).mem_ground_left
+      simp only [restrict_ground_eq, restrict_cl_eq', image_val_inter_self_left_eq_coe,
+        preimage_union, preimage_inter, Subtype.coe_preimage_self, inter_univ, preimage_diff]
+      intro Z
+      rw [image_image, cl_image_of_forall_parallel'_subtype _ h_para, image_image]
+      have hYE : Y ⊆ M.E := fun y hy ↦ by simpa using (h_para (φ.symm ⟨y,hy⟩)).mem_ground_right
+
+      simp [preimage_val_eq_univ_of_subset hXE, diff_eq_empty.2 hYE]
+      ext x
+      simp only [mem_inter_iff, mem_image, mem_preimage, Subtype.exists, exists_and_left]
+      refine ⟨fun ⟨hx,hxY⟩  ↦ ⟨φ.symm ⟨_,hxY⟩, ?_⟩, ?_⟩
+      · simp only [Subtype.coe_eta, Equiv.apply_symm_apply, Subtype.coe_prop, exists_const, and_true]
+        exact mem_of_mem_of_subset (by simpa using (h_para (φ.symm ⟨x,hxY⟩)).mem_cl) <|
+          M.cl_subset_cl_of_subset_cl (by simpa)
+      rintro ⟨x, hx', hx, rfl⟩
+      simp only [Subtype.coe_prop, and_true]
+      exact mem_of_mem_of_subset (h_para ⟨x,hx⟩).symm.mem_cl <|
+          M.cl_subset_cl_of_subset_cl (by simpa) )
+
+/-- If `φ` is a permutation of `M.E` that maps each element to something `Parallel'`, then
+`φ` determines an automorphism of `M`. -/
+def isoOfMapParallel (φ : M.E ≃ M.E) (h_para : ∀ (e : M.E), M.Parallel' e (φ e)) : M ≂ M :=
+  let ψ := (Iso.ofEq <| M.restrict_ground_eq_self)
+  ψ.symm.trans (Iso.trans (isoOfMapParallelRestr φ h_para) ψ)
+
+/-- If `φ : α → α` restricts to a permutation of `M.E` and maps each element to something
+`Parallel'`, it induces an automorphism of `M`. -/
+@[simps] noncomputable def isoOfMapParallelBijOn {φ : α → α} (hφ : BijOn φ M.E M.E)
+    (h_para : ∀ e ∈ M.E, M.Parallel' e (φ e)) : M ≂ M where
+  toEquiv := hφ.equiv
+  indep_image_iff' I := (isoOfMapParallel hφ.equiv (by simpa [BijOn.equiv])).indep_image_iff
+
+@[simp] theorem isoOfMapParallelBijOn_apply {φ} (hφ : BijOn φ M.E M.E)
+    (h_para : ∀ e ∈ M.E, M.Parallel' e (φ e)) (x : M.E) :
+    isoOfMapParallelBijOn hφ h_para x = ⟨φ x, (h_para x.1 x.2).mem_ground_right⟩ := rfl
+
+@[simp] theorem isoOfMapParallelBijOn_apply_image {φ} (hφ : BijOn φ M.E M.E)
+    (h_para : ∀ e ∈ M.E, M.Parallel' e (φ e)) (X : Set M.E) :
+    isoOfMapParallelBijOn hφ h_para '' X = φ '' X := by
+  suffices ∀ (x y : α) (h : y ∈ M.E), ⟨y, h⟩ ∈ X → φ y = x → x ∈ M.E by simpa [Set.ext_iff]
+  rintro x y h - rfl
+  exact (h_para y h).mem_ground_right
+
+end Iso
+
+section Swap
+
+/-- Swapping two `Parallel'` matroid elements gives an automorphism -/
+@[simps!] noncomputable def isoOfSwapParallel [DecidableEq α] (h_para : M.Parallel' e f) : M ≂ M :=
+  isoOfMapParallelBijOn (φ := Equiv.swap e f)
+    (Equiv.swap_bijOn_self (iff_of_true h_para.mem_ground_left h_para.mem_ground_right))
+    (by
+      intro x hx
+      obtain (rfl | he) := eq_or_ne x e; simpa
+      obtain (rfl | hf) := eq_or_ne x f; simpa using h_para.symm
+      rw [Equiv.swap_apply_of_ne_of_ne he hf]
+      exact M.parallel'_self hx )
+
+@[simp] theorem isoOfSwapParallel_apply [DecidableEq α] (h_para : M.Parallel' e f) (x : M.E) :
+    isoOfSwapParallel h_para x = ⟨Equiv.swap e f x, (isoOfSwapParallel h_para x).2⟩ := rfl
+
+@[simp] theorem isoOfSwapParallel_apply_image [DecidableEq α] (h_para : M.Parallel' e f)
+    (X : Set M.E) : isoOfSwapParallel h_para '' X = Equiv.swap e f '' X := by
+  rw [isoOfSwapParallel, isoOfMapParallelBijOn_apply_image]
+
+theorem Indep.parallel_substitute (hI : M.Indep I) (h_para : M.Parallel' e f)
+    (heI : e ∈ I) : M.Indep (insert f (I \ {e})) := by
+  classical
+  convert (isoOfSwapParallel h_para).image_indep (I := M.E ↓∩ I)
+    (by rwa [image_val_preimage_val_of_subset hI.subset_ground])
+  simp only [isoOfSwapParallel_apply_image, Subtype.image_preimage_coe,
+    inter_eq_self_of_subset_right hI.subset_ground]
+  by_cases hfI : f ∈ I
+  · obtain (rfl : e = f) := h_para.eq_of_indep (hI.subset (pair_subset heI hfI))
+    simpa
+  rw [(Equiv.swap_bijOn_exchange heI hfI).image_eq]
+
+theorem Parallel.indep_substitute_iff (h_para : M.Parallel' e f) (he : e ∈ I) (hf : f ∉ I) :
+    M.Indep I ↔ M.Indep (insert f (I \ {e})) := by
+  refine ⟨fun hI ↦ hI.parallel_substitute h_para he, fun hI ↦ ?_⟩
+  convert hI.parallel_substitute h_para.symm (mem_insert _ _)
+  have hef : e ≠ f := by rintro rfl; exact hf he
+  simp [insert_diff_singleton_comm hef, insert_eq_of_mem he, diff_singleton_eq_self hf]
+
+end Swap
+
+section Subtype
+
+variable {φ : I → α}
+
+theorem indep_iff_range_indep_of_paraMap {φ : I → α} (hφ : φ.Injective)
+    (h_para : ∀ e : I, M.Parallel' e (φ e)) : M.Indep I ↔ M.Indep (range φ) := by
+  set ψ := Equiv.ofInjective _ hφ
+  convert Iso.indep_image_iff (I := univ) <|
+    (isoOfMapParallelRestr ψ (by simpa only [Equiv.ofInjective_apply, ψ] using h_para)) using 1
+  · simp [Subset.rfl]
+  simp only [restrict_ground_eq, image_univ, restrict_indep_iff, image_subset_iff,
+    Subtype.coe_preimage_self, subset_univ, and_true]
+  simp_rw [← image_univ, image_image, image_univ]
+  rfl
+
+end Subtype
+
+section Function
+
+theorem Indep.paraMap_injective (hI : M.Indep I) (φ : I → α)
+    (h_para : ∀ e : I, M.Parallel' e (φ e)) : φ.Injective := by
+  intro x y hxy
+  have hx := h_para x
+  rw [hxy] at hx
+  exact Subtype.val_inj.1
+    ((hx.trans (h_para y).symm).eq_of_indep (hI.subset (pair_subset x.2 y.2)))
+
+theorem Indep.indep_range_paraMap (hI : M.Indep I) (φ : I → α)
+    (h_para : ∀ e : I, M.Parallel' e (φ e)) : M.Indep (range φ) := by
+  rwa [← indep_iff_range_indep_of_paraMap (hI.paraMap_injective φ h_para) h_para]
+
+theorem Indep.image_paraMap {φ : α → α} (hI : M.Indep I) (h_para : ∀ e ∈ I, M.Parallel' e (φ e)) :
+    M.Indep (φ '' I) := by
+  convert hI.indep_range_paraMap (fun e ↦ φ e) (by simpa); simp [Set.ext_iff]
+
+theorem Indep.of_image_paraMap {φ : α → α} (hI : M.Indep (φ '' I)) (hφ : InjOn φ I)
+    (h_para : ∀ e ∈ I, M.Parallel' e (φ e)) : M.Indep I := by
+  rwa [indep_iff_range_indep_of_paraMap hφ.injective (by simpa), range_restrict]
+
+theorem indep_image_iff_of_injOn_paraMap {φ : α → α} (hφ : InjOn φ I)
+    (h : ∀ e ∈ I, M.Parallel' e (φ e)) : M.Indep (φ '' I) ↔ M.Indep I :=
+  ⟨fun hI ↦ hI.of_image_paraMap hφ h, fun hi ↦ hi.image_paraMap h⟩
+
+end Function
+
+
+section ParallelClass
+
+theorem mem_parallelClasses_iff_eq_cl_diff_loops {P : Set α} :
+    P ∈ M.parallelClasses ↔ ∃ e, M.Nonloop e ∧ P = M.cl {e} \ M.cl ∅ := by
+  simp only [parallelClasses, Partition.mem_congr_iff, Flat.mem_covbyPartition_iff,
+    loops_covby_iff, point_iff_exists_eq_cl_nonloop]
+  constructor
+  · rintro ⟨_, ⟨e, he, rfl⟩, rfl⟩
+    exact ⟨e, he, rfl⟩
+  rintro ⟨e, he, rfl⟩
+  exact ⟨_, ⟨e, he, rfl⟩,rfl⟩
+
+theorem mem_parallelClasses_iff {P : Set α} :
+    P ∈ M.parallelClasses ↔ ∃ e, M.Nonloop e ∧ P = {f | M.Parallel e f} := by
+  simp_rw [mem_parallelClasses_iff_eq_cl_diff_loops, setOf_parallel_eq_cl_diff_loops]
+
+@[simp] theorem parallelClasses_partOf_eq (M : Matroid α) (e : α) :
+    M.parallelClasses.partOf e = {f | M.Parallel e f} :=
+  (M.parallelClasses.setOf_rel_eq_partOf e).symm
+
+/-- Parallel classes correspond to points -/
+@[simps] def parallelPointEquiv (M : Matroid α) :
+    ↑ (M.parallelClasses)  ≃ {P // M.Point P} where
+  toFun P := ⟨P ∪ M.cl ∅, by
+    obtain ⟨e, he, h⟩ := mem_parallelClasses_iff_eq_cl_diff_loops.1 P.prop
+    rw [h, diff_union_self, union_eq_self_of_subset_right (M.cl_subset_cl (empty_subset _))]
+    exact he.cl_point ⟩
+  invFun P := ⟨P \ M.cl ∅, by
+    obtain ⟨e, he, heP⟩ := P.prop.exists_eq_cl_nonloop
+    rw [mem_parallelClasses_iff_eq_cl_diff_loops]
+    exact ⟨e, he, by rw [heP]⟩⟩
+  left_inv := by
+    rintro ⟨P, hP⟩
+    obtain ⟨e, -, rfl⟩ := mem_parallelClasses_iff_eq_cl_diff_loops.1 hP
+    simp
+  right_inv := by
+    rintro ⟨P, hP⟩
+    obtain ⟨e, -, rfl⟩ := hP.exists_eq_cl_nonloop
+    simp
+
+end ParallelClass
+
+section Series
+
+section Series
+
+def Series (M : Matroid α) (e f : α) : Prop := M✶.Parallel e f
+
+-- API TODO, but all will follow easily from duality.
+
+
+end Series
